Logic/Modal/Standard/Kripke/Preservation.lean
@@ -91,6 +91,25 @@ infix:80 " →ₚ " => Frame.PseudoEpimorphism
 instance : CoeFun (Frame.PseudoEpimorphism F₁ F₂) (λ _ => F₁.World → F₂.World) := ⟨λ f => f.toFun⟩
 
 
+def Frame.PseudoEpimorphism.TransitiveClosure {F₁ F₂ : Frame} (f : F₁ →ₚ F₂) (F₂_trans : Transitive F₂) : F₁^+ →ₚ F₂ where
+  toFun := f.toFun
+  forth := by
+    intro x y hxy; simp at x y;
+    induction hxy with
+    | single hxy => exact f.forth hxy;
+    | @tail z y _ Rzy Rxz =>
+      replace Rzy := f.forth Rzy;
+      exact F₂_trans Rxz Rzy;
+  back := by
+    intro x w hxw;
+    obtain ⟨u, ⟨rfl, hxu⟩⟩ := f.back hxw;
+    use u;
+    constructor;
+    . rfl;
+    . exact RelTransGen.single hxu;
+
+
+
 structure Model.PseudoEpimorphism (M₁ M₂ : Kripke.Model α) extends M₁.Frame →ₚ M₂.Frame where
   atomic {w : M₁.World} {a} : (M₁.Valuation w a) ↔ (M₂.Valuation (toFun w) a)
 
@@ -189,6 +208,125 @@ theorem undefinable_irreflexive : ¬∃ (Ax : AxiomSet α), AxiomSet.DefinesKrip
   contradiction;
 
 end PseudoEpimorphism
+
+
+
+section
+
+def Frame.isRooted (F : Frame) (r : F.World) : Prop := ∀ w ≠ r, r ≺ w
+
+
+structure RootedFrame extends Kripke.Frame where
+  root : World
+  root_rooted : Frame.isRooted _ root
+  default := root
+
+
+variable [DecidableEq α]
+
+open Relation (TransGen ReflTransGen)
+
+def Frame.PointGenerated (F : Kripke.Frame) (r : F.World) : Kripke.Frame where
+  World := { w | w = r ∨ r ≺ w }
+  Rel x y := x.1 ≺ y.1
+  default := ⟨r, by tauto⟩
+
+namespace Frame.PointGenerated
+
+variable {F : Kripke.Frame} {r : F.World}
+
+lemma rel_transitive (F_trans : Transitive F) : Transitive (F.PointGenerated r).Rel := by
+  rintro ⟨x, (rfl | hx)⟩ ⟨y, (rfl | hy)⟩ ⟨z, (rfl | hz)⟩ hxy hyz;
+  all_goals aesop;
+
+lemma rel_irreflexive (F_irrefl : Irreflexive F) : Irreflexive (F.PointGenerated r).Rel := by
+  rintro ⟨x, (rfl | hx)⟩ h;
+  all_goals aesop;
+
+lemma rooted : (F.PointGenerated r).isRooted ⟨r, by tauto⟩ := by
+  rintro ⟨x, (rfl | hx)⟩;
+  . intro h; contradiction;
+  . intro _; exact hx;
+
+end Frame.PointGenerated
+
+
+abbrev Frame.PointGenerated' (F : Kripke.Frame) (r : F.World) : Kripke.RootedFrame :=
+  letI G := F.PointGenerated r;
+  {
+    World := G.World
+    Rel := G.Rel
+    root := ⟨r, by tauto⟩
+    root_rooted := by simpa using @Frame.PointGenerated.rooted F r
+  }
+infix:100 "↾" => Frame.PointGenerated'
+
+lemma Frame.PointGenerated'.rel_transitive {F : Kripke.Frame} {r : F.World} : Transitive F → Transitive (F↾r).Rel := PointGenerated.rel_transitive
+
+lemma Frame.PointGenerated'.rel_irreflexive {F : Kripke.Frame} {r : F.World} : Irreflexive F → Irreflexive (F↾r).Rel := PointGenerated.rel_irreflexive
+
+
+def Model.PointGenerated (M : Kripke.Model α) (r : M.World) : Kripke.Model α where
+  Frame := (M.Frame↾r).toFrame
+  Valuation w a := M.Valuation w.1 a
+infix:100 "↾" => Model.PointGenerated
+
+def Model.PointGenerated.Bisimulation (M : Model α) (M_trans : Transitive M.Frame) (r : M.World) : (M↾r) ⇄ M where
+  toRel x y := x.1 = y
+  atomic := by
+    rintro x y a rfl;
+    simp [Model.PointGenerated];
+  forth := by
+    rintro x₁ y₁ x₂ rfl Rx₂y₁;
+    use y₁.1;
+    constructor;
+    . simp;
+    . exact Rx₂y₁;
+  back := by
+    rintro ⟨x₁, (rfl | hx₁)⟩ x₂ y₂ rfl Rx₂y₂;
+    . use ⟨y₂, by right; exact Rx₂y₂⟩;
+      constructor;
+      . simp;
+      . exact Rx₂y₂;
+    . use ⟨y₂, ?h₂⟩;
+      constructor;
+      . simp;
+      . exact Rx₂y₂;
+      right;
+      exact M_trans hx₁ Rx₂y₂;
+
+lemma Model.PointGenerated.Bisimulation.rooted (M_trans : Transitive M.Frame := by assumption) : (Bisimulation M M_trans r) ⟨r, by simp⟩ r := by simp [Bisimulation];
+
+lemma Model.PointGenerated.modal_equivalent_to_root (M : Model α) (M_trans : Transitive M.Frame) (r : M.World) : ModalEquivalent (M₁ := M↾r) (M₂ := M) ⟨r, by simp⟩ r
+  := modal_equivalent_of_bisimilar (Bisimulation M M_trans r) Bisimulation.rooted
+
+
+namespace Frame
+
+variable {F : Kripke.Frame} (x : F.World)
+
+def successors := { w // x ≺^* w }
+postfix:100 "↑*" => Frame.upward
+
+def immediate_successors := { w // x ≺ w }
+postfix:100 "↑¹" => Frame.immediate_successor
+
+def proper_immediate_successors := { w // x ≠ w ∧ x ≺ w }
+postfix:100 "↑" => Frame.proper_immediate_successor
+
+
+def predeccsors := { w // w ≺^* x }
+postfix:100 "↓*" => Frame.downward
+
+def immediate_predeccsors := { w // w ≺ x }
+postfix:100 "↓¹" => Frame.immediate_predeccsor
+
+def proper_immediate_predeccsors := { w // w ≠ x ∧ w ≺ x }
+postfix:100 "↓" => Frame.proper_immediate_predeccsors
+
+end Frame
+
+end
 
 end Kripke
 
