Logic/Modal/Standard/Kripke/Kripke.lean
@@ -3,9 +3,14 @@ import Logic.Modal.Standard.Kripke.Completeness
 import Logic.Modal.Standard.Kripke.Preservation
 import Logic.Modal.Standard.Kripke.Filteration
 
+import Logic.Modal.Standard.Kripke.ComplexityLimited
+
 import Logic.Modal.Standard.Kripke.Geach
 import Logic.Modal.Standard.Kripke.Ver
 import Logic.Modal.Standard.Kripke.Dot3
+import Logic.Modal.Standard.Kripke.S5
 import Logic.Modal.Standard.Kripke.GL
+-- TODO: move
+import Logic.Modal.Standard.Kripke.GL_tree
 
 import Logic.Modal.Standard.Kripke.ModalCompanion
